Include adequacy result.

examples/store/game.v
@@ -6,7 +6,7 @@ From iris.algebra Require Import agree auth csum gset gmap excl frac.
 From iris.algebra Require Import numbers reservation_map.
 From iris.heap_lang Require Import notation proofmode adequacy.
 From iris.heap_lang.lib Require Import par assert ticket_lock.
-From cryptis Require Import cryptis primitives tactics gmeta role.
+From cryptis Require Import cryptis primitives tactics gmeta role adequacy.
 From cryptis.primitives Require Import attacker.
 From cryptis.examples Require Import iso_dh rpc gen_conn conn store.
 
@@ -34,9 +34,7 @@ Definition start_server : val := λ: "c" "skR",
   let: "server" := Server.start "skR" in
   server_loop "c" "server".
 
-Definition game : val := λ: <>,
-  let: "c" := init_network #() in
-
+Definition game : val := λ: "c",
   (* Create key pairs and give verification keys to attacker *)
   let: "skI" := mk_sign_key #() in
   let: "skR" := mk_sign_key #() in
@@ -94,13 +92,13 @@ iIntros "%ss server". wp_pures.
 wp_apply (wp_server_loop with "[$server]"); eauto.
 Qed.
 
-Lemma wp_game :
+Lemma wp_game c :
   cryptis_ctx -∗
+  channel c -∗
   store_ctx -∗
-  WP game #() {{ _, True }}.
+  WP game c {{ _, True }}.
 Proof.
-iIntros "#ctx #store_ctx"; rewrite /game; wp_pures.
-wp_apply wp_init_network => //. iIntros "%c #cP". wp_pures.
+iIntros "#ctx #chan #store_ctx"; rewrite /game; wp_pures.
 wp_apply (wp_mk_sign_key with "[]"); eauto.
 iIntros "%skI #m_skI s_skI tokenI". wp_pures.
 wp_pures. wp_apply (wp_mk_sign_key with "[]"); eauto.
@@ -147,20 +145,19 @@ End Game.
 Definition F : gFunctors :=
   #[heapΣ; spawnΣ; cryptisΣ; tlockΣ; iso_dhΣ; GenConn.connΣ; RPC.rpcΣ; storeΣ].
 
-Lemma store_secure σ₁ σ₂ (v : val) t₂ e₂ :
-  rtc erased_step ([game #()], σ₁) (t₂, σ₂) →
+Lemma store_secure σ₁ σ₂ t₂ e₂ :
+  rtc erased_step ([run_network game], σ₁) (t₂, σ₂) →
   e₂ ∈ t₂ →
   not_stuck e₂ σ₂.
 Proof.
 have ? : heapGpreS F by apply _.
 apply (adequate_not_stuck NotStuck _ _ (λ v _, True)) => //.
-apply: heap_adequacy.
-iIntros (?) "?".
-iMod (cryptisGS_alloc _) as (?) "(#ctx & _ & sign_tok & senc_tok & _)".
+apply: cryptis_adequacy.
+iIntros (? ? c) "#ctx #chan (_ & sign_tok & senc_tok & _)".
 iMod (iso_dhGS_alloc with "sign_tok") as (?) "(#? & iso_tok & sign_tok)" => //.
 iMod (Conn.pre_ctx_alloc with "[//] [$]") as "(#? & senc_tok)" => //.
 iMod (RPC.ctx_alloc with "[//] [$]") as (?) "(#? & iso_tok & rpc_tok)" => //.
 iMod (store_ctx_alloc with "[$] [//]") as "(#? & rpc_tok)";
   first solve_ndisj.
-by iApply (wp_game with "ctx [//]") => //.
+by iApply (wp_game with "ctx chan [//]") => //.
 Qed.
